AP/Determinacy.lean
@@ -23,97 +23,33 @@ theorem game₀_state' {pw a d} : (game₀ pw a d).toState' = state'₀ pw := rf
 def AState.a_hws (s : AState) := ∃ a, ∀ d, (s.to_game a d).a_wins
 def AState.d_hws (s : AState) := ∃ d, ∀ a, (s.to_game a d).d_wins
 
-theorem a_state_move'_of_move {sa : AState} {sd}
-(h : sa.move sd) : sa.move' sd := h.1
+#check 0 #exit
 
-theorem d_state_move'_of_move {sd : DState} {sa}
-(h : sd.move sa) : sd.move' sa := h.1
-
-theorem game_le_of_play_size_eq_size_add {g : Game} {n x}
-(h : (g.play n).size = g.size + x) : x ≤ n := by
-  by_contra! h₁
-  obtain ⟨k, rfl⟩ := Nat.exists_eq_add_of_lt h₁
-  clear h₁
-  have h₁ := @game_play_size_lt_iff_play_ended g n
-  by_cases h₂ : (g.play n).ended <;> simp [h₂] at h₁
-  · by_cases h₃ : g.ended
-    · rw [game_play_eq_of_ended h₃] at h
-      simp at h
-    · specialize h₁ h₃
-      rw [h] at h₁
-      linarith
-  rw [game_play_size_eq_of_not_ended h₂] at h
-  linarith
-
-theorem game_play_size_eq_self_of_any {g : Game} {n x}
-(h : (g.play n).size = g.size + x) : (g.play x).size = g.size + x := by
-  obtain ⟨k, rfl⟩ := Nat.exists_eq_add_of_le # game_le_of_play_size_eq_size_add h
-  simp at h
-  by_cases he : (g.play x).ended
-  · simp [game_play_eq_of_ended he] at h
-    exact h
-  apply game_play_size_eq_of_not_ended he
-
-theorem game₀_play_size_eq_self_of_any {pw a d x} (n : ℕ)
-(h : ((game₀ pw a d).play n).size = x) : ((game₀ pw a d).play x).size = x := by
-  generalize hg : game₀ pw a d = g at *
-  replace h : (g.play n).size = g.size + x :=
-    by
-      nth_rewrite 2 [←hg]
-      simpa
-  replace h := game_play_size_eq_self_of_any h
-  nth_rewrite 2 [←hg] at h
-  simp at h
-  exact h
-
-def d_state₀ (pw : ℕ) : DState := by
-  refine' ⟨⟨state₀ pw, _⟩, _⟩ <;> simp
-
-def a_state₀ (pw : ℕ) : AState :=
-  Classical.epsilon (d_state₀ pw).move
-
-@[simp]
-theorem d_state₀_toState_eq {pw} : (d_state₀ pw).toState = state₀ pw := rfl
-
-@[simp]
-theorem state_mk_size {s' hist} : (⟨s', hist⟩ : State).size = hist.length := rfl
+theorem a_state_move_of_move' {sa : AState} {sd : DState}
+(h : sa.move' sd) : sa.move sd := by
+  unfold AState.move' at h
+  obtain ⟨⟨⟨s₂', h₃⟩, h₄⟩, h₁, h₂⟩ := exi_a_state_move_of_a_move h
+  obtain ⟨⟨s₂, h₅⟩, h₆⟩ := sd
+  dsimp at h h₁ h₄ h₆
+  convert h₂
+  obtain ⟨h₂, h₇⟩ := h₂
+  dsimp at h₇
+  rw [h₇]
+  unfold AState.move' at h₂
+  dsimp at h₂
 
 #check 0 #exit
 
-theorem exi_d_state₀_move {pw} : ∃ sa, (d_state₀ pw).move sa := by
-  have ⟨s, hs⟩ := d_always_has_move #
-    state'_valid_of_state_valid (d_state₀ pw).h_valid
-  dsimp only [d_state₀] at hs
-  refine' ⟨⟨⟨⟨s, [state'₀ pw]⟩, _⟩, _⟩, _⟩
-  · have ⟨g, hg⟩ := hv # game₀ pw default #
-      mk_strat_const s
-    refine' ⟨g.move, _, _⟩; simp [hg]
-    simp [hg, Game.move]
-    rw [strat_set_ap_of_eq hs]
-    rfl
-  · simp
-  · unfold DState.move
-
-#check 0 #exit
-
-theorem exi_a_state_move : ∃ (sa : AState) (sd : DState), sa.move sd := by
-  obtain ⟨⟨s, g, ⟨pw, a, d, n, rfl⟩, rfl⟩, h⟩ := exi_valid_state_with_size 2
-  dsimp at h
-  generalize hg₀ : game₀ pw a d = g₀ at h; rw [eq_comm] at hg₀
-  obtain ⟨g, hg⟩ := hv # g₀.play 2
-  have h₁ : g.size = 2 :=
-    by
-      subst hg₀ hg
-      exact game₀_play_size_eq_self_of_any n h
-  rw [exists_swap]
-  use d_state₀ pw
+theorem a_state_move'_iff_move {sa : AState} {sd : DState} :
+sa.move' sd ↔ sa.move sd := ⟨a_state_move_of_move', a_state_move'_of_move⟩
 
 #check 0 #exit
 
 theorem not_a_state_move'_imp_move :
 ¬∀ (sa : AState) (sd : DState), sa.move' sd → sa.move sd := by
   push_neg
-  use default
+  obtain ⟨sa, sd, h⟩ := exi_a_state_move
+  obtain ⟨sd₁, hsd₁⟩ := hv # ({sd with hist := []} : DState)
 
 #check 0 #exit
 
